steel/formats/lowstar/Zeta.LowStar.Parser.fst
@@ -31,3 +31,27 @@ let parser (#t:Type0) (p:spec_parser t) =
          | _ -> False
          end
        )
+
+let len_offset_ok (a:byte_array)
+                  (len:U32.t)
+                  (offset:U32.t) =
+  B.length a == U32.v len /\
+  U32.v offset < U32.v len
+
+inline_for_extraction
+let serializer (#t:Type0) (#p:spec_parser t) (s:spec_serializer p) =
+    len:U32.t ->
+    offset:U32.t ->
+    a:byte_array { len_offset_ok a len offset } ->
+    v:t { Seq.length (s v) <= U32.v len - U32.v offset } ->
+    HST.Stack U32.t
+        (requires (fun h ->
+          B.live h a
+        ))
+        (ensures (fun h slice_len h' ->
+          let bs = B.as_seq h' a in
+          B.modifies (B.loc_buffer a) h h' /\
+          U32.v slice_len == Seq.length (s v) /\
+          len_offset_slice_ok a len offset slice_len /\
+          Seq.length bs == (U32.v len <: nat) /\
+          s v == slice bs offset slice_len ))
