steel/formats/spec/Zeta.Steel.LogEntry.Spec.fst
@@ -73,3 +73,45 @@ let runapp_payload_offset
   runapp_payload_offset' e
 
 #pop-options
+
+let synth_stamped_record
+  (x: Zeta.Formats.Aux.Stamped_record.stamped_record)
+: Tot Zeta.Steel.LogEntry.Types.stamped_record
+= {
+  Zeta.Steel.LogEntry.Types.record = Zeta.Formats.Synth.synth_record x.sr_record;
+  Zeta.Steel.LogEntry.Types.timestamp = x.sr_timestamp;
+  Zeta.Steel.LogEntry.Types.thread_id = x.sr_thread_id;
+}
+
+let synth_stamped_record_recip
+  (x: Zeta.Steel.LogEntry.Types.stamped_record)
+: Tot Zeta.Formats.Aux.Stamped_record.stamped_record
+= {
+  sr_record = Zeta.Formats.Synth.synth_record_recip x.Zeta.Steel.LogEntry.Types.record;
+  sr_timestamp = x.Zeta.Steel.LogEntry.Types.timestamp;
+  sr_thread_id = x.Zeta.Steel.LogEntry.Types.thread_id;
+}
+
+module LPC = LowParse.Spec.Combinators
+
+let spec_parser_stamped_record' =
+  LPC.parse_synth
+    Zeta.Formats.Aux.Stamped_record.stamped_record_parser
+    synth_stamped_record
+
+let spec_parser_stamped_record x =
+  match LPC.parse spec_parser_stamped_record' x with
+  | None -> None
+  | Some (res, consumed) -> Some (res, consumed)
+
+let spec_serializer_stamped_record' : LPC.serializer spec_parser_stamped_record' =
+  LPC.serialize_synth
+    _
+    synth_stamped_record
+    Zeta.Formats.Aux.Stamped_record.stamped_record_serializer
+    synth_stamped_record_recip
+    ()
+
+let spec_serializer_stamped_record x = LPC.serialize spec_serializer_stamped_record' x
+
+let serialized_stamped_record_length s = ()
