steel/formats/steel/Zeta.Steel.FormatsLib.fst
@@ -42,3 +42,61 @@ let mk_steel_parser
 = fun len offset slice_len a ->
   let b = read_bytes len offset slice_len a _ () in
   p32 b
+
+let rec write_bytes
+    (alen: Ghost.erased U32.t)
+    (offset:U32.t)
+    (b: Ghost.erased (Seq.seq U8.t))
+    (new_bytes: FStar.Bytes.bytes)
+    (a:A.array U8.t)
+    (sq: squash (
+      U32.v offset + FStar.Bytes.length new_bytes <= Seq.length b /\
+      Seq.length b == U32.v alen
+    ))
+:   S.ST (Ghost.erased (Seq.seq U8.t))
+       (A.pts_to a Steel.FractionalPermission.full_perm b)
+       (fun b' -> A.pts_to a Steel.FractionalPermission.full_perm b')
+       (requires True)
+       (ensures fun b' ->
+         let offset' = U32.v offset + FStar.Bytes.length new_bytes in
+         Seq.length b' == Seq.length b /\
+         (forall (i: nat { i < Seq.length b }) . {:pattern Seq.index b' i}
+           Seq.index b' i == (if U32.v offset <= i && i < offset' then FStar.Bytes.index new_bytes (i - U32.v offset) else Seq.index b i))
+       )
+=
+  let len = FStar.Bytes.len new_bytes in
+  if len = 0ul
+  then
+    S.return b
+  else begin
+    let r = FStar.Bytes.get new_bytes 0ul in
+    A.write a offset r;
+    write_bytes alen (offset `U32.add` 1ul) (Seq.upd b (U32.v offset) r) (FStar.Bytes.sub new_bytes 1ul (len `U32.sub` 1ul)) a ()
+  end
+
+let mk_steel_serializer
+  (#k: LP.parser_kind)
+  (#t: Type)
+  (#p: LP.parser k t)
+  (#s: LP.serializer p)
+  (s32: LP.serializer32 s)
+  (#p0: P.spec_parser t)
+  (s0: P.spec_serializer p0)
+  (s0_eq: squash (forall (x: t) . s0 x `Seq.equal` s x))
+: Tot (P.serializer s0)
+= fun len offset a v ->
+  let new_bytes = s32 v in
+  let slice_len = FStar.Bytes.len new_bytes in
+  let b : Ghost.erased (Seq.seq P.byte) = S.elim_exists #_ #_ #(Zeta.Steel.Util.array_pts_to a) () in
+  A.pts_to_length #_ #_ #Steel.FractionalPermission.full_perm a b;
+  let b' : Ghost.erased (Seq.seq P.byte) = write_bytes len offset b new_bytes a () in
+  assert (s0 v `Seq.equal` P.slice b' offset slice_len);
+  S.intro_pure _;
+  S.intro_exists_erased b' (fun (bs: Seq.seq P.byte) ->
+              Zeta.Steel.Util.array_pts_to a bs `S.star`
+              S.pure (
+                U32.v slice_len == Seq.length (s0 v) /\
+                P.len_offset_slice_ok a len offset slice_len /\
+                Seq.length bs == (U32.v len <: nat) /\
+                s0 v == P.slice bs offset slice_len ));
+  S.return slice_len
