steel/formats/steel/Zeta.Steel.LogEntry.fst
@@ -30,3 +30,15 @@ let parse32_log_entry
 
 let parser_log_entry =
   Zeta.Steel.FormatsLib.mk_steel_parser parse32_log_entry spec_parser_log_entry ()
+
+let serialize32_stamped_record : LowParse.SLow.Base.serializer32 spec_serializer_stamped_record' =
+  LowParse.SLow.Combinators.serialize32_synth'
+    _
+    synth_stamped_record
+    _
+    Zeta.Formats.Aux.Stamped_record.stamped_record_serializer32
+    synth_stamped_record_recip
+    ()
+
+let serialize_stamped_record =
+  Zeta.Steel.FormatsLib.mk_steel_serializer serialize32_stamped_record spec_serializer_stamped_record ()
