steel/formats/lowstar/Zeta.LowStar.LogEntry.fsti
@@ -3,3 +3,5 @@ open Zeta.Steel.LogEntry.Spec
 open Zeta.LowStar.Parser
 
 val parser_log_entry : parser spec_parser_log_entry
+
+val serialize_stamped_record : serializer spec_serializer_stamped_record
